````col
```col-md

```
```col-md
aw
```
````

$$
\begin{aligned}
 & f(x) = x^{4} + 3x + 1 \\
 & f(-1) = 1 - 3 + 1 = -1 < 0 \\
 & f(-2) = 16 - 6 + 1 = 11 > 0 \\
 & \text{By I.V.T.,}\ \exists c_{1} :  \\
 & f(c_{1}) = 0,\ -2 < c_{1} < -1 \\ \\
 & \text{Suppose an assumption}\ A: \exists c_{2}:  \\
 & f(c_{2}) = 0,\ -2 < c_{2} < -1 \\
 & \text{By M.V.T.,}\ \exists c_{3}: \\
 & f'(c_{3}) = \frac{f(c_{1}) - f(c_{2})}{c_{1}-c_{2}} = 0, \\
 & c_{1}<c_{3}<c_{2} \lor c_{2} < c_{3} < c_{1} \\
 & \implies -2 < c_{3} < -1 \\ \\
 & f'(x) = 4x^{3} + 3,\ f''(x) = 12x^{2} \\
 & \forall x \in \mathbb{R},\ f''(x) \ge 0,\ f'(x)\ \text{increases} \\
 & f'(-1) = -4 + 3 < 0 \\
 & \implies \forall x < -1,\ f'(x) < 0,\ f(x)\ \text{decreases}
\end{aligned}
$$