$$
\begin{aligned} \text{let}\ g(x) = f(x)|_{x = x_{0}}  & + f'(x) | _{x=x_{0}} (x - x_{0})  \\
 & + \frac{1}{2} f''(x)|_{x=x_{0}} (x - x_{0})^{2}  \\
 & + \frac{1}{3!} f^{(3)}(x)_{x=x_{0}}(x-x_{0})^{3} + \dots \\
 & = \sum ^{\infty}_{k = 0} \frac{f^{(k)}(x_{0})}{k!}(x-x_{0})^{k}
\end{aligned}
$$
$$
\begin{aligned}
 & g(x_{0}) = f(x_{0}), \\
 & g'(x) = f'(x_{0}), \\
 & g''(x) = f''(x_{0})\dots
\end{aligned}
$$
By Tylor expansion we can get **a good approximation** of a function.
In general, we only need to do the first and second layer of expansion to get an approximation function that is neat enough in practice.