$$
\begin{aligned}
 & - \frac{GMm}{3R} + \frac{1}{2}m{v_{1}}^{2} = - \frac{GMm}{6R} + \frac{1}{2}m{v_{2}}^{2} \\
 & \to g = \frac{GM}{R^{2}},\ \frac{GM}{R} = gR,\  -\frac{1}{3}gR + \frac{1}{2}{v_{1}}^{2} = -\frac{1}{6}gR + \frac{1}{2}{v_{2}}^{2} \\
 & \cancel{\frac{1}{2}}({v_{1}}^{2}-{v_{2}}^{2}) = 2\cdot \left( -\frac{1}{6} + \frac{1}{3} \right)gR,\ {v_{1}}^{2}-{v_{2}}^{2} = 2\cdot \frac{1}{6}gR = \frac{1}{3}gR \\
 & ----- \\
 & 3R\cdot m\cdot v_{1} = 6R\cdot m\cdot v_{2} \to v_{1} = 2v_{2} \\
 & ----- \\
 & {v_{2}}^{2}(4-1) = 3{v_{2}}^{2} = \frac{1}{3}gR,\ v_{2} = \sqrt{ \frac{1}{9}gR } = \frac{1}{3}\sqrt{ gR } \\
 & L = m\cdot 6R\cdot \frac{1}{3}\sqrt{ gR } = 2mR\sqrt{ gR }\ \blacksquare
\end{aligned}
$$

$$
\frac{1}{5} + \frac{1}{6} = \frac{11}{30}
$$
$$
\frac{1}{6} + \frac{1}{4} = \frac{10}{24} = \frac{5}{12}
$$


----

$\alpha \beta \gamma \delta \epsilon \varepsilon \nu \mu \sigma \phi \chi \rho \varphi \omega\theta\iota \eta \kappa\lambda \zeta \phi$

$$
\mathrm{
\tau\epsilon \mu \pi \omega \rho\alpha \rho\upsilon
}\ \
\theta \epsilon\ \theta \iota \nu \gamma\ \iota\sigma\ \gamma\epsilon \tau \tau\iota \nu\gamma\ o\upsilon \tau\ o\phi\ \kappa o\nu \tau \rho o\lambda.\ \ \ \omega\epsilon\ \mu\upsilon\sigmaC \tau\ \nu o\tau\ \upsilon \nu \delta\epsilon \rho\varepsilon \sigma \tau\iota \mu\alpha \tau\epsilon\ \iota \tau.

$$
$$
E(X) = 1 \implies E(X^{5}) = E^{5}(X) = 1^{5} = 1\ \blacksquare
$$
$$
\begin{pmatrix}
1 & 0 & 0 \\
0 & 1 & 0 \\
0 & 0 & 1
\end{pmatrix}\cdot \begin{pmatrix}
a & b & c \\
d & e & f \\
g & h & i
\end{pmatrix} = \begin{pmatrix}
a & b & c \\
d & e & f \\
g & h & i
\end{pmatrix}
$$
