# 9.1
16.
$$
a_{n} = \frac{(-1)^{n - 1}}{n^{2}}\ \blacksquare
$$
45.
$$
\begin{aligned}
 & a_{n} = \sqrt{ \frac{2n}{n + 1} }. \\
 & \text{Assume that }a_{n}\ \text{converges, then} \\
 & \lim_{ n \to \infty } a_{n} = \sqrt{ \lim_{ n \to \infty } \frac{2n}{n+1} } \\
 & = \sqrt{ \lim_{ n \to \infty } \frac{2n}{n} } = \sqrt{ 2 }\ \blacksquare
\end{aligned}
$$
53.
$$
\begin{aligned}
 & \text{By L'Hopital's Rule: } \\
 & \begin{aligned}
\lim_{ n \to \infty } a_{n} & = \lim_{ n \to \infty } \frac{\ln(n + 1)}{\sqrt{ n }} \\
 & = \lim_{ n \to \infty } \frac{[\ln(n+1)]'}{(\sqrt{ n })'} \\
 & = \lim_{ n \to \infty } \frac{\frac{1}{n+1}}{\frac{1}{2n}} = \lim_{ n \to \infty } \frac{2n}{n+1} = 2\ \blacksquare
\end{aligned}
\end{aligned}
$$
64.
$$
\begin{aligned}
 & a_{n} = \ln n - \ln (n + 1) = \ln \frac{n}{n+1} \\
 & \begin{aligned}
\lim_{ n \to \infty } a_{n} & = \lim_{ n \to \infty } \ln \frac{n}{n+1} \\
 & = \ln \lim_{ n \to \infty } \frac{n}{n+1} \\
 & = \ln 1 = 0\ \blacksquare
\end{aligned}
\end{aligned}
$$
65.
$$
\begin{aligned}
 & a_{n} = \sqrt[ n ]{ 4^{n}n } = 4\cdot \sqrt[ n ]{ n } = 4n^{1/n} \\
 & \ln a_{n} = \ln 4 + \frac{1}{n} \ln n \\
 & \begin{aligned}
\lim_{ n \to \infty } \ln a_{n} & = \ln 4 + \lim_{ n \to \infty } \frac{1}{n}\ln n \\
 & = \ln 4 + \lim_{ n \to \infty } \frac{(\ln n )'}{n'} \\
 & = \ln 4 + \lim_{ n \to \infty } \frac{1}{n} = \ln 4
\end{aligned} \\
 & \lim_{ n \to \infty } a_{n} = e^{\ln 4} = 4\ \blacksquare
\end{aligned}
$$
115.
a
$$
\begin{aligned}
 & \text{By L'Hopital's Theorem, }  \\
 & \lim_{ n \to \infty } \frac{\ln n}{n^{c}} = \lim_{ x \to \infty } \frac{(\ln x)'}{(x^{c})'} = \lim_{ x \to \infty } \frac{\frac{1}{x}}{cx^{c-1}} = \lim_{ x \to \infty } \frac{1}{cx^{c}} = c\cdot \lim_{ n \to \infty } \frac{1}{n^{c}} = 0\ \blacksquare
\end{aligned}
$$
b
$$
\begin{aligned}
 & \left| \frac{1}{n^{c}} - 0 \right| = \frac{1}{n^{c}} < \varepsilon,\ n^{c} > \varepsilon ^{-1},\ n > \varepsilon ^{-1/c} \\
 & (\forall \varepsilon \in \mathbb{Z}^{+})(N \in \varepsilon ^{-1/c})n > N \implies \left| a_{n} - L  \right|  = \left|  \frac{1}{n^{c}} - 0  \right| = \frac{1}{n^{c}} < \varepsilon \ \blacksquare
\end{aligned}
$$
# 9.2
3
$$
\begin{aligned}
 & \text{let}\ r = -\frac{1}{2},\ a_{1} = 1 \\
 & S_{n} = \frac{1 - r^{n}}{1 - r} = \frac{1 - \left( -\frac{1}{2} \right)^{n}}{1 + \frac{1}{2}} \\
 & S = \lim_{ n \to \infty } S_{n} = \frac{1}{\frac{3}{2}} = \frac{2}{3}\ \blacksquare
\end{aligned}
$$
5
$$
\begin{aligned}
 & \frac{1}{(n+1)(n+2)} = \frac{1}{n+1} - \frac{1}{n+2} \\
 & \begin{aligned}
S_{n} & = \left( \frac{1}{2} - \frac{1}{3} \right) + \left( \frac{1}{3} - \frac{1}{4} \right) + \dots + \left( \frac{1}{n} - \frac{1}{n + 1} \right) + \left( \frac{1}{n+1} - \frac{1}{n+2} \right) \\
 & = \frac{1}{2} - \frac{1}{n+2}
\end{aligned} \\
 & S = \lim_{ n \to \infty } S_{n} = \frac{1}{2}\ \blacksquare
\end{aligned}
$$
11
$$
\begin{aligned}
 & <a_{n}>\ = \left\{  \frac{5}{2}+\frac{1}{3},\ \frac{5}{4} + \frac{1}{9},\ \frac{5}{8} + \frac{1}{27},\ \frac{5}{16} + \frac{1}{81},\ \frac{5}{32} + \frac{1}{243},\ \frac{5}{64} + \frac{1}{729},\ \frac{5}{128} + \frac{1}{2187},\ \frac{5}{256} + \frac{1}{6561}  \right\} \\
 & \sum ^{\infty}_{n = 1} \left( \frac{5}{2^{n}} + \frac{1}{3^{n}} \right) = \sum ^{\infty}_{n = 1} \frac{5}{2^{n}} + \sum ^{\infty}_{n = 1} \frac{1}{3^{n}} = \frac{5}{1 - \frac{1}{2}} + \frac{1}{1 - \frac{1}{3}} = 10 + \frac{3}{2} = \frac{23}{2}\ \blacksquare
\end{aligned}
$$
32
$$
\begin{aligned}
 & \lim_{ n \to \infty } \frac{n ( n + 1)}{(n + 2)(n + 3)} = \lim_{ n \to \infty } \frac{n^{2} + n}{n^{2} + 5n + 6} = 1 \ne 0 \\
 & \therefore \sum ^{\infty}_{n = 1} \frac{n ( n+1)}{(n + 2)(n + 3)}\ \text{diverges}\ \blacksquare
\end{aligned}
$$
34
$$
\begin{aligned}
 & \lim_{ n \to \infty } \frac{n}{n^{2} + 3} = 0 \therefore \text{the test is inconclusive}\ \blacksquare
\end{aligned}
$$
38
$$
\begin{aligned}
 & \lim_{ n \to \infty } \cos n \pi\  \text{diverges} \\
 & \implies \because \text{limit fails to exist}\ \therefore \text{summation diverges}\ \blacksquare
\end{aligned}
$$
46
$$
\begin{aligned}
 & \frac{1}{2n - 1} - \frac{1}{2n + 1} = \frac{2n + 1 - (2n - 1)}{(2n - 1)(2n + 1)} = \frac{2}{(2n - 1)(2n + 1)} \\
  & \begin{aligned}
\sum ^{\infty}_{n = 1} \frac{6}{(2n - 1)(2n + 1)} & = \sum ^{\infty}_{n = 1}\left( \frac{3}{2n - 1} - \frac{3}{2n + 1} \right) \\
 & = \left( \frac{3}{1} - \frac{3}{3} \right) + \left( \frac{3}{3} - \frac{3}{5} \right) + \dots \\
 & + \left( \frac{3}{2n - 3} - \frac{3}{2n - 1} \right) + \left( \frac{3}{2n - 1} - \frac{3}{2n + 1} \right) \\
 & = \lim_{ n \to \infty } \left( 3 - \frac{3}{2n + 1} \right) = 3\ \blacksquare
\end{aligned}
\end{aligned}
$$

48
$$
\begin{aligned}
 & \frac{1}{n^{2}} - \frac{1}{(n + 1)^{2}} = \frac{n^{2} + 2n + 1 - n^{2}}{n^{2}(n+1)^{2}} = \frac{2n + 1}{n^{2}(n+1)^{2}} \\
 &  \begin{aligned}
 \implies \sum ^{\infty}_{n = 1} \frac{2n + 1}{n^{2}(n + 1)^{2}}  & = \left(  \frac{1}{1} - \frac{1}{4} \right) + \left( \frac{1}{4} - \frac{1}{9} \right) + \dots \\
 & + \left( \frac{1}{(n - 1)^{2}} - \frac{1}{n^{2}} \right) + \left( \frac{1}{n^{2}} - \frac{1}{(n + 1)^{2}} \right) + \dots\\
 & = \lim_{ n \to \infty } \left( 1 - \frac{1}{(n + 1)^{2}} \right) = 1\ \blacksquare
\end{aligned}
\end{aligned}
$$
58
$$
\begin{aligned}
 & \because \cos n \pi \le 1 \therefore \sum ^{\infty}_{n = 0} \frac{1}{5^{n}} \ge \sum ^{\infty}_{n = 0} \frac{\cos n \pi}{5^{n}}, \\
 & \sum ^{\infty}_{n = 0} \frac{1}{5^{n}} = \frac{1}{1- \frac{1}{5}} = \frac{5}{4} \implies \sum ^{\infty}_{n = 0} \frac{\cos n \pi}{5^{n}} \le \frac{5}{4} < \infty \therefore \text{converges}  \\
 & < \frac{\cos (n - 1)\pi}{5^{n - 1}} >\ = \left\{  1, -\frac{1}{5},\ \frac{1}{25},\ - \frac{1}{125},\ \dots, \ \frac{\cos(n-1)\pi}{5^{n-1}}  \right\} \\
 & \text{let}\ a = 1,\ r = - \frac{1}{5}: \frac{\cos (n - 1)\pi}{5^{n - 1}} = 1\cdot \left( -\frac{1}{5} \right)^{n - 1} = ar^{n - 1} \\
 & \because \left| r \right| < 1 \therefore \sum ^{\infty}_{n = 1}ar^{n - 1}= \frac{1}{1-r} = \frac{5}{6}\ \blacksquare
\end{aligned}
$$
66
$$
\begin{aligned}
 & < \frac{n^{n}}{n!} > \ = \left\{   \frac{1}{1},\ \frac{2 \times 2}{1 \times 2},\ \frac{3 \times 3\times 3}{1 \times 2 \times 3},\ \dots  \right\} \\
 & \lim_{ n \to \infty } \frac{n^{n}}{n!} \text{diverges}\ \therefore \sum ^{\infty}_{n = 1} \frac{n^{n}}{n!}\ \text{diverges too}\ \blacksquare
\end{aligned}
$$

72
$$
\begin{aligned}
 & \frac{e^{n\pi}}{\pi ^{ne}} = \left( \frac{e^{\pi}}{\pi ^{e}} \right)^{n} \\
 & \text{Note that}\ \ln e^{\pi} = \pi,\ \ln \pi ^{e} = e \ln \pi \\
 & \text{let}\ f(x) = x,\ g(x) = e \ln x \implies \pi = f(\pi),\ e \ln \pi = g(\pi) \\
 & \text{Analyzing functions}:\  \\
 & \text{1.}\ f(e) = g(e) = e \\
 & \text{2.}\ f'(x) = 1,\ g'(x) = \frac{e}{x};\ g'(e) = \frac{e}{e} = 1;\ g'(x) < 1 \\
 & \therefore \forall x > e,\ g(x) < f(x) \\
 & \because \pi > e \therefore g(\pi) < f(\pi) \\
 & \to e \ln \pi < \pi \ln e \\
 & \to \pi ^{e} < e^{\pi} \\
 & \to \frac{e^{\pi}}{\pi ^{e}} > 1 \\
 & \therefore \sum ^{\infty}_{n = 0} \left( \frac{e^{\pi}}{\pi ^{e}} \right)^{n}\ \text{diverges}\ \blacksquare
\end{aligned}
$$
# 9.3
6
$$
\begin{aligned}
 & \frac{1}{x(\ln x)^{2}} \ \text{is continuous, positive and decreasing function for all } x \ge 2\\
 &  \int ^{\infty}_{2} \frac{1}{x (\ln x)^{2}}\ dx = \int ^{\infty}_{\ln 2} \frac{1}{(\ln x)^{2}}\ d\ln x = - \left( \frac{1}{\ln x} \right)^{\infty}_{\ln 2}\ \therefore \text{converges}\ \blacksquare
\end{aligned}
$$
7
$$
\begin{aligned}
 & \frac{x}{x^{2} + 4}\ \text{is continuous, positive and decreasing function for all}\ x \ge 1 \\
 & \int ^{\infty}_{1} \frac{x}{x^{2}+4} \ dx = \int ^{\infty}_{1} \frac{dx^{2}}{2(x^{2} + 4) } = \int ^{\infty}_{1} \frac{d(x^{2} + 4)}{2(x^{2} + 4)} = \ln(x^{2} + 4)|^{\infty}_{1} \therefore \text{diverges}\ \blacksquare
\end{aligned}
$$

43
$$
\sum ^{\infty}_{n = 1} \frac{ 8 \tan ^{-1} n}{1 + n^{2}}
$$
$$
\begin{aligned}
 & \text{Applying integral test:} \\
 & \begin{aligned}
 \int ^{\infty}_{1} \frac{8 \tan ^{-1} x}{1 + x^{2}} \ dx & = \int ^{\infty}_{1} 8 \tan ^{-1} x \ d(\tan ^{-1} x) \\
 & = 4 \tan ^{-1} x |^{\infty}_{1} \\
 & = 4\left( \frac{\pi}{2} - \frac{\pi}{4} \right) = \pi
\end{aligned} \\
 & \therefore \int ^{\infty}_{1} \frac{8 \tan ^{-1} x}{1 + x^{2}}\ dx \ \text{converges} \implies \sum ^{\infty}_{n = 1} \frac{8 \tan ^{-1} n}{1 + n^{2}}\ \text{converges too}\ \blacksquare
\end{aligned}
$$