# 9.1
10.
$$
a_{n} = \frac{(-1)^{n - 1}}{n^{2}}\ \blacksquare
$$
45.
$$
\begin{aligned}
 & a_{n} = \sqrt{ \frac{2n}{n + 1} }. \\
 & \text{Assume that }a_{n}\ \text{converges, then} \\
 & \lim_{ n \to \infty } a_{n} = \sqrt{ \lim_{ n \to \infty } \frac{2n}{n+1} } \\
 & = \sqrt{ \lim_{ n \to \infty } \frac{2n}{n} } = \sqrt{ 2 }\ \blacksquare
\end{aligned}
$$
53.
$$
\begin{aligned}
 & \text{By L'Hopital's Rule: } \\
 & \begin{aligned}
\lim_{ n \to \infty } a_{n} & = \lim_{ n \to \infty } \frac{\ln(n + 1)}{\sqrt{ n }} \\
 & = \lim_{ n \to \infty } \frac{[\ln(n+1)]'}{(\sqrt{ n })'} \\
 & = \lim_{ n \to \infty } \frac{\frac{1}{n+1}}{\frac{1}{2n}} = \lim_{ n \to \infty } \frac{2n}{n+1} = 2\ \blacksquare
\end{aligned}
\end{aligned}
$$
64.
$$
\begin{aligned}
 & a_{n} = \ln n - \ln (n + 1) = \ln \frac{n}{n+1} \\
 & \begin{aligned}
\lim_{ n \to \infty } a_{n} & = \lim_{ n \to \infty } \ln \frac{n}{n+1} \\
 & = \ln \lim_{ n \to \infty } \frac{n}{n+1} \\
 & = \ln 1 = 0\ \blacksquare
\end{aligned}
\end{aligned}
$$
65.
$$
\begin{aligned}
 & a_{n} = \sqrt[ n ]{ 4^{n}n } = 4\cdot \sqrt[ n ]{ n } = 4n^{1/n} \\
 & \ln a_{n} = \ln 4 + \frac{1}{n} \ln n \\
 & \begin{aligned}
\lim_{ n \to \infty } \ln a_{n} & = \ln 4 + \lim_{ n \to \infty } \frac{1}{n}\ln n \\
 & = \ln 4 + \lim_{ n \to \infty } \frac{(\ln n )'}{n'} \\
 & = \ln 4 + \lim_{ n \to \infty } \frac{1}{n} = \ln 4
\end{aligned} \\
 & \lim_{ n \to \infty } a_{n} = e^{\ln 4} = 4\ \blacksquare
\end{aligned}
$$
**TODO**
# 9.2
3
$$
\begin{aligned}
 & \text{let}\ r = -\frac{1}{2},\ a_{1} = 1 \\
 & S_{n} = \frac{1 - r^{n}}{1 - r} = \frac{1 - \left( -\frac{1}{2} \right)^{n}}{1 + \frac{1}{2}} \\
 & S = \lim_{ n \to \infty } S_{n} = \frac{1}{\frac{3}{2}} = \frac{2}{3}\ \blacksquare
\end{aligned}
$$
5
$$
\begin{aligned}
 & \frac{1}{(n+1)(n+2)} = \frac{1}{n+1} - \frac{1}{n+2} \\
 & \begin{aligned}
S_{n} & = \left( \frac{1}{2} - \frac{1}{3} \right) + \left( \frac{1}{3} - \frac{1}{4} \right) + \dots + \left( \frac{1}{n} - \frac{1}{n + 1} \right) + \left( \frac{1}{n+1} - \frac{1}{n+2} \right) \\
 & = \frac{1}{2} - \frac{1}{n+2}
\end{aligned} \\
 & S = \lim_{ n \to \infty } S_{n} = \frac{1}{2}\ \blacksquare
\end{aligned}
$$
11
$$
\begin{aligned}
 & <a_{n}>\ = \left\{  \frac{5}{2}+\frac{1}{3},\ \frac{5}{4} + \frac{1}{9},\ \frac{5}{8} + \frac{1}{27},\ \frac{5}{16} + \frac{1}{81},\ \frac{5}{32} + \frac{1}{243},\ \frac{5}{64} + \frac{1}{729},\ \frac{5}{128} + \frac{1}{2187},\ \frac{5}{256} + \frac{1}{6561}  \right\} \\
 & \sum ^{\infty}_{n = 1} \left( \frac{5}{2^{n}} + \frac{1}{3^{n}} \right) = \sum ^{\infty}_{n = 1} \frac{5}{2^{n}} + \sum ^{\infty}_{n = 1} \frac{1}{3^{n}} = \frac{5}{1 - \frac{1}{2}} + \frac{1}{1 - \frac{1}{3}} = 10 + \frac{3}{2} = \frac{23}{2}\ \blacksquare
\end{aligned}
$$
32
$$
\begin{aligned}
 & \lim_{ n \to \infty } \frac{n ( n + 1)}{(n + 2)(n + 3)} = \lim_{ n \to \infty } \frac{n^{2} + n}{n^{2} + 5n + 6} = 1 \ne 0 \\
 & \therefore \sum ^{\infty}_{n = 1} \frac{n ( n+1)}{(n + 2)(n + 3)}\ \text{diverges}\ \blacksquare
\end{aligned}
$$
34
$$
\lim_{ n \to \infty } \cos n \pi\ \text{is divergent}\implies \sum ^{\infty}_{n = 1} \cos n \pi\ \text{diverges}\ \blacksquare
$$
46
$$
\begin{aligned}
 & \frac{1}{2n - 1} - \frac{1}{2n + 1} = \frac{2n + 1 - (2n - 1)}{(2n - 1)(2n + 1)} = \frac{2}{(2n - 1)(2n + 1)} \\
  & \begin{aligned}
\sum ^{\infty}_{n = 1} \frac{6}{(2n - 1)(2n + 1)} & = \sum ^{\infty}_{n = 1}\left( \frac{3}{2n - 1} - \frac{3}{2n + 1} \right) \\
 & = \left( \frac{3}{1} - \frac{3}{3} \right) + \left( \frac{3}{3} - \frac{3}{5} \right) + \dots \\
 & + \left( \frac{3}{2n - 3} - \frac{3}{2n - 1} \right) + \left( \frac{3}{2n - 1} - \frac{3}{2n + 1} \right) \\
 & = \lim_{ n \to \infty } \left( 3 - \frac{3}{2n + 1} \right) = 3\ \blacksquare
\end{aligned}
\end{aligned}
$$

48
$$
\begin{aligned}
 & \frac{1}{n^{2}} - \frac{1}{(n + 1)^{2}} = \frac{n^{2} + 2n + 1 - n^{2}}{n^{2}(n+1)^{2}} = \frac{2n + 1}{n^{2}(n+1)^{2}} \\
 &  \begin{aligned}
 \implies \sum ^{\infty}_{n = 1} \frac{2n + 1}{n^{2}(n + 1)^{2}}  & = \left(  \frac{1}{1} - \frac{1}{4} \right) + \left( \frac{1}{4} - \frac{1}{9} \right) + \dots \\
 & + \left( \frac{1}{(n - 1)^{2}} - \frac{1}{n^{2}} \right) + \left( \frac{1}{n^{2}} - \frac{1}{(n + 1)^{2}} \right) + \dots\\
 & = \lim_{ n \to \infty } \left( 1 - \frac{1}{(n + 1)^{2}} \right) = 1\ \blacksquare
\end{aligned}
\end{aligned}
$$
