# 6.1
26
$$
\begin{aligned}
V & = \pi\int ^{\pi/4}_{-\pi / 4} \sec ^{2} x\ dx \\
 & = 2\pi \int ^{\pi / 4}_{0} \sec ^{2}x\ dx \\
 & = 2\pi \tan x\ |^{\pi/4}_{0} \\
 & = 2\pi(1 - 0) = 2\pi\ \blacksquare
\end{aligned}
$$
28
$$
\begin{aligned}
V & = \pi\int ^{\pi/2}_{\pi/6} \cot x\ dx \\
 & = \pi\ln \left| \sin x \right| ^{\pi /2}_{\pi / 6} \\
 & = \pi \left(\ln 1 - \ln \frac{1}{2}\right) = \pi\ln \frac{1}{\frac{1}{2}} = \pi\ln 2\ \blacksquare
\end{aligned}
$$
29
$$
\begin{aligned}
V & = \pi\int ^{4}_{1/4} \left( \frac{1}{2\sqrt{ x }} \right)^{2}\ dx \\
 & = \pi \int ^{4}_{1 / 4} \frac{1}{4x}\ dx \\
 & = \frac{\pi}{4}\ln \left| x \right| ^{4}_{1 / 4} \\
 & = \frac{\pi}{4}\left( \ln 4 - \ln \frac{1}{4} \right) \\
 & = \frac{\pi}{4}\ln 16 = \pi \ln 2\ \blacksquare
\end{aligned}
$$
37
$$
\begin{aligned}
V & = \pi \int ^{3}_{0}\left( \frac{2}{\sqrt{ y + 1 }} \right)^{2}\ dy \\
 & = \pi \int ^{3}_{0} \frac{4}{y + 1}\ dy \\
 & = \pi \int ^{3}_{0} \frac{4}{y + 1}\ d(y + 1) \\
 & = 4\pi \ln \left| y + 1 \right| ^{3}_{0} \\
 & = 4\pi(\ln 4 - \ln 1) \\
 & = 8\pi \ln 2\ \blacksquare
\end{aligned}
$$
38
$$
\begin{aligned}
V & = \pi\int ^{1}_{0} \left( \frac{\sqrt{ 2y }}{y^{2} + 1} \right)^{2}\ dy \\
 & = \pi \int ^{1}_{0} \frac{2y}{(y^{2} + 1)}\ dy \\
 & = \pi \int ^{1}_{0} \frac{dy^{2}}{y^{2} + 1} \\
 & = \pi \int ^{1}_{0} \frac{d(y^{2} + 1)}{y^{2} + 1} \\
 & = \pi \ln \left| y^{2} + 1 \right| ^{1}_{0} \\
 & = \pi \ln 2\ \blacksquare
\end{aligned}
$$
50
$$
\begin{aligned}
 & x^{2} + y^{2} = 3,\ y = \pm \sqrt{ 3 - x^{2} } \\
 & \begin{aligned}
V & = \pi\int ^{\sqrt{ 3 }}_{0} (\sqrt{ 3 })^{2} - (\sqrt{ 3 - x^{2} })^{2}\ dx \\
 & = \pi \int ^{\sqrt{ 3 }}_{0} x^{2}\ dx \\
 & = \frac{\pi}{3}x^{3}\ |^{\sqrt{ 3 }}_{0} = \pi \sqrt{ 3 }\ \blacksquare
\end{aligned}
\end{aligned}
$$
